Rename output_events --> io_events (better for paper)

examples/divScript.sml
@@ -478,8 +478,8 @@ val _ = process_topdecs `
 
 val st = ml_translatorLib.get_ml_prog_state();
 
-val output_events_def = Define `
-  output_events = SIO [||]`;
+val io_events_def = Define `
+  io_events = SIO [||]`;
 
 val _ = overload_on("yes",``yes_v``);
 
@@ -487,13 +487,13 @@ Theorem yes_spec:
   !uv.
     limited_parts names p ==>
     app (p:'ffi ffi_proj) ^(fetch_v "yes" st) [arg]
-      (output_events []) (POSTd io. io = LREPEAT [put_str_event "y\n"])
+      (io_events []) (POSTd io. io = LREPEAT [put_str_event "y\n"])
 Proof
   xcf_div "yes" st
   \\ MAP_EVERY qexists_tac
     [`K emp`, `\i. REPLICATE_LIST [put_str_event "y\n"] i`, `K ($= arg)`,
      `K (State [||])`, `update`]
-  \\ fs [GSYM SIO_def, REPLICATE_LIST_def, output_events_def]
+  \\ fs [GSYM SIO_def, REPLICATE_LIST_def, io_events_def]
   \\ xsimpl \\ rw [lprefix_lub_def]
   THEN1 (
     xlet `POSTv v. &UNIT_TYPE () v *
